additive linear logic with both kinds of quantifiers

formulas.v
@@ -1,7 +1,8 @@
 (* Formulas with separated first- and second-order quantifiers *)
 
 From Coq Require Import Lia.
-From Quantifiers Require Export foterms.
+From OLlibs Require Import List_more.
+From Quantifiers Require Export foterms_ext.
 
 Set Implicit Arguments.
 
@@ -16,7 +17,8 @@ Arguments evar _ _ {T}.
 Notation evar := (evar vatom tatom).
 
 Notation "r ;; s" := (fecomp r s) (at level 20, format "r  ;;  s").
-Notation closed t := (tvars t = nil).
+Notation tclosed t := (tvars t = nil).
+Notation rtclosed r := (forall n, tclosed (r n)).
 Notation "⇑" := fup.
 Notation "⇑[ u ] r" := (felift u r) (at level 25, format "⇑[ u ] r").
 
@@ -24,19 +26,17 @@ Hint Rewrite (@tesubs_evar vatom tatom) : term_db.
 Hint Rewrite (@tesubs_comp vatom tatom) : term_db.
 Hint Rewrite (@tsubs_tsubs_eq vatom tatom) : term_db.
 Hint Rewrite (@tsubs_tsubs vatom tatom)
-                        using try (intuition; fail);
-                             (try apply closed_notvars); intuition; fail : term_db.
-Hint Rewrite (@tvars_tesubs_fclosed vatom tatom) using intuition; fail : term_db.
-Hint Rewrite (@tvars_tsubs_closed vatom tatom) using intuition; fail : term_db.
+                        using try tauto;
+                              try apply closed_notvars; tauto : term_db.
+Hint Rewrite (@tvars_tesubs_closed vatom tatom) using tauto : term_db.
+Hint Rewrite (@tvars_tsubs_closed vatom tatom) using tauto : term_db.
 Hint Rewrite (@notin_tsubs vatom tatom)
-                         using try easy;
-                              (try (intuition; fail));
-                              (try apply closed_notvars); intuition; fail : term_db.
+                         using try easy; try tauto;
+                               try apply closed_notvars; tauto: term_db.
 Hint Rewrite (@notin_tsubs_bivar vatom tatom)
-                               using try easy;
-                                    (try (intuition; fail));
-                                    (try apply closed_notvars); intuition; fail : term_db.
-Hint Rewrite (@tsubs_tesubs vatom tatom) using try (intuition; fail) : term_db.
+                               using try easy; try tauto;
+                                     try apply closed_notvars; tauto : term_db.
+Hint Rewrite (@tsubs_tesubs vatom tatom) using try tauto : term_db.
 
 Hint Resolve tesubs_ext : term_db.
 Hint Resolve closed_notvars : term_db.
@@ -82,40 +82,64 @@ Ltac formula_induction A :=
   let lll := fresh "l" in
   let tt := fresh "t" in
   let IHll := fresh "IHl" in
-  induction A as [ n | XX | RR ll | ncon | ucon A ? | bcon A1 ? A2 ?
-                 | qcon xx A | qcon XX A ]; simpl; intros;
-  [ try (apply (f_equal sevar)); try ((rnow idtac) ; fail)
-  | try (apply (f_equal svar)); repeat case_analysis; try ((rnow idtac) ; fail)
+  let IH := fresh "IH" in
+  let IH2 := fresh "IH" in
+  induction A as [ n | XX | RR ll | ncon | ucon A IH | bcon A1 IH A2 IH2
+                 | qcon xx A IH | qcon XX A IH ]; simpl; intros;
+  [ try (apply (f_equal sevar)); try ((rnow idtac); fail)
+  | try (apply (f_equal svar)); repeat case_analysis; try ((rnow idtac); fail)
   | rewrite ? flat_map_concat_map;
     try (apply (f_equal (fvar _)));
     try (induction ll as [ | tt lll IHll ]; simpl; intuition;
          rewrite IHll; f_equal; intuition)
-  | try ((try f_equal); intuition; fail)
+  | try (try f_equal; intuition; fail)
   | try (apply (f_equal (funa _))); intuition
   | try (apply (f_equal2 (fbin _))); intuition
-  | (try apply (f_equal (fqtf _ _))); repeat case_analysis; try (intuition; fail);
-     try (now rcauto)
-  | (try apply (f_equal (sqtf _ _))); repeat case_analysis; try (intuition; fail);
-     try (now rcauto) ];
-  try (now rcauto).
+  | (try apply (f_equal (fqtf _ _))); repeat case_analysis; try (intuition; fail); try now rcauto
+  | (try apply (f_equal (sqtf _ _))); repeat case_analysis; try (intuition; fail); try now rcauto ];
+  try (rewrite ? IH, ? IH2; reflexivity);
+  try now rcauto.
+
+(** * Atomic formulas *)
+
+Inductive atomic U T : formula U T -> Prop :=
+| atomic_sevar u : atomic (sevar u)
+| atomic_svar X : atomic (svar X)
+| atomic_fvar f l : atomic (fvar f l).
 
 
 (** * Size of [formula] *)
 
 Fixpoint fsize U T (A : formula U T) :=
 match A with
-| sevar _ => 1
-| svar _ => 1
-| fvar _ _ => 1
-| fnul _ => 1
+| sevar _ | svar _ | fvar _ _ | fnul _ => 1
 | funa _ B => S (fsize B)
 | fbin _ B C => S (fsize B + fsize C)
-| fqtf _ _ B => S (fsize B)
-| sqtf _ _ B => S (fsize B)
+| fqtf _ _ B | sqtf _ _ B => S (fsize B)
 end.
 
 
 (** * Free variables in [formula] *)
+
+Fixpoint freevars U T (A : formula U T) :=
+match A with
+| sevar _ => nil
+| svar _ => nil
+| fvar _ l => flat_map (@tvars _ _ _) l
+| fnul _ => nil
+| funa _ B => freevars B
+| fbin _ B C => freevars B ++ freevars C
+| fqtf _ x B => remove eq_dt_dec x (freevars B)
+| sqtf _ x B => freevars B
+end.
+Notation fclosed A := (freevars A = nil).
+Notation rfclosed r := (forall n, fclosed (r n)).
+
+Lemma fclosed_nofreevars U T (A : formula U T) x : fclosed A -> ~ In x (freevars A).
+Proof. intros -> []. Qed.
+
+Lemma rfclosed_nofreevars U1 U2 T (r : U1 -> formula U2 T) n x : rfclosed r -> ~ In x (freevars (r n)).
+Proof. intros -> []. Qed.
 
 Fixpoint sfreevars U T (A : formula U T) :=
 match A with
@@ -129,6 +153,13 @@ match A with
 | sqtf _ X B => remove eq_dt_dec X (sfreevars B)
 end.
 Notation sclosed A := (sfreevars A = nil).
+Notation rsclosed r := (forall n, sclosed (r n)).
+
+Lemma sclosed_nosfreevars U T (A : formula U T) X : sclosed A -> ~ In X (sfreevars A).
+Proof. intros -> []. Qed.
+
+Lemma rsclosed_nosfreevars U1 U2 T (r : U1 -> formula U2 T) n x : rsclosed r -> ~ In x (sfreevars (r n)).
+Proof. intros -> []. Qed.
 
 
 (** * Substitution of first-order eigen variables in [formula] *)
@@ -151,6 +182,24 @@ Notation "A ⟦ r ⟧" := (esubs r A) (at level 8, left associativity, format "A
 Lemma fsize_esubs U T1 T2 (r : T1 -> term T2) (A : formula U T1) : fsize A⟦r⟧ = fsize A.
 Proof. formula_induction A. Qed.
 Hint Rewrite fsize_esubs : term_db.
+
+Lemma freevars_esubs_closed U T1 T2 (r : T1 -> term T2) (A : formula U T1) (Hc : rtclosed r) :
+  freevars A⟦r⟧ = freevars A.
+Proof. formula_induction A. Qed.
+Hint Rewrite freevars_esubs_closed using tauto : term_db.
+
+Lemma freevars_esubs U T1 T2 (r : T1 -> term T2) (A : formula U T1) : incl (freevars A) (freevars A⟦r⟧).
+Proof. formula_induction A.
+- clear. induction l as [|t l IHl]; cbn; [ intro; tauto | ].
+  apply incl_app_app, IHl.
+  apply tvars_tesubs.
+- apply remove_incl. assumption.
+Qed.
+#[local] Hint Rewrite freevars_esubs : term_db.
+
+Lemma sfreevars_esubs U T1 T2 (r : T1 -> term T2) (A : formula U T1) : sfreevars A⟦r⟧ = sfreevars A.
+Proof. formula_induction A. Qed.
+#[local] Hint Rewrite sfreevars_esubs : term_db.
 
 Lemma esubs_evar U T (A : formula U T) : A⟦evar⟧ = A.
 Proof. formula_induction A. Qed.
@@ -189,8 +238,18 @@ Definition fescomp U1 U2 U3 T (r : U1 -> formula U2 T) (s : U2 -> formula U3 T) 
 Notation "r ;2; s" := (fescomp r s) (at level 20, format "r  ;2;  s").
 
 Lemma fsize_essubs U1 U2 T (r : U1 -> formula U2 T) A : fsize A <= fsize A⟦r⟧2.
-Proof. formula_induction A; (try (destruct (r n))); simpl; lia. Qed.
+Proof. formula_induction A; (try (destruct (r n))); cbn; lia. Qed.
 Hint Rewrite fsize_essubs : term_db.
+
+Lemma freevars_essubs_closed U1 U2 T (r : U1 -> formula U2 T) (A : formula U1 T) (Hc : rfclosed r) :
+  freevars A⟦r⟧2 = freevars A.
+Proof. formula_induction A. Qed.
+#[local] Hint Rewrite freevars_essubs_closed : term_db.
+
+Lemma sfreevars_essubs_closed U1 U2 T (r : U1 -> formula U2 T) (A : formula U1 T) (Hc : rsclosed r) :
+  sfreevars A⟦r⟧2 = sfreevars A.
+Proof. formula_induction A. Qed.
+#[local] Hint Rewrite sfreevars_essubs_closed : term_db.
 
 Lemma essubs_evar U T (A : formula U T) : A⟦sevar⟧2 = A.
 Proof. formula_induction A. Qed.
@@ -225,7 +284,17 @@ Notation "A [ u // x ]" := (subs x u A) (at level 8, format "A [ u // x ]").
 
 Lemma fsize_subs U T u x (A : formula U T) : fsize A[u//x] = fsize A.
 Proof. formula_induction A. Qed.
-Hint Rewrite fsize_subs : term_db.
+#[local] Hint Rewrite fsize_subs : term_db.
+
+Lemma nfree_subs U T x u (A : formula U T) : ~ In x (freevars A) -> subs x u A = A.
+Proof. formula_induction A.
+- apply notin_tsubs. intro. apply H. in_solve.
+- apply H. in_solve.
+- apply IH. intro. apply H. apply in_in_remove; auto.
+Qed.
+#[local] Hint Rewrite nfree_subs using try tauto;
+                                       try (apply fclosed_nofreevars; tauto);
+                                       try apply rfclosed_nofreevars; tauto : term_db.
 
 
 (** ** Substitution of second-order variables in [formula] *)
@@ -246,38 +315,85 @@ end.
 Notation "A [ F // X ]2" := (ssubs X F A) (at level 8, format "A [ F // X ]2").
 
 Lemma fsize_ssubs U T F X (A : formula U T) : fsize A <= fsize A[F//X]2.
-Proof. formula_induction A; (try destruct F); simpl; lia. Qed.
-Hint Rewrite fsize_ssubs : term_db.
+Proof. formula_induction A; (try destruct F); cbn; lia. Qed.
+#[local] Hint Rewrite fsize_ssubs : term_db.
 
+Lemma fsize_ssubs_atomic U T F X (A : formula U T) : atomic F -> fsize A[F//X]2 = fsize A.
+Proof. formula_induction A; (try destruct F; inversion H); cbn; lia. Qed.
+#[local] Hint Rewrite fsize_ssubs_atomic : term_db.
 
 (** ** Additional results with variable eigen type *)
 
-Lemma subs_esubs U T1 T2 (r : T1 -> term T2) x u (A : formula U T1): (forall n, closed (r n)) ->
+Lemma nfree_ssubs U T X F (A : formula U T) : ~ In X (sfreevars A) -> A[F//X]2 = A.
+Proof. formula_induction A. apply IH. intro. apply H. apply in_in_remove; auto. Qed.
+#[local] Hint Rewrite nfree_ssubs using try tauto;
+                                       try (apply sclosed_nosfreevars; tauto);
+                                       try apply rsclosed_nosfreevars; tauto : term_db.
+
+Lemma subs_esubs U T1 T2 (r : T1 -> term T2) x u (A : formula U T1): rtclosed r ->
   A[u//x]⟦r⟧ = A⟦r⟧[tesubs r u//x].
-Proof. formula_induction A; simpl in H; rcauto. Qed.
-Hint Rewrite subs_esubs using intuition; fail : term_db.
+Proof. formula_induction A. Qed.
+#[local] Hint Rewrite subs_esubs using tauto : term_db.
 
-Lemma notin_ssubs U T X (F A : formula U T) : ~ In X (sfreevars A) -> A[F//X]2 = A.
-Proof. formula_induction A; apply IHA; intros Hv; apply H, in_in_remove; auto. Qed.
-Hint Rewrite notin_ssubs using try easy;
-                              (try (intuition; fail)); intuition; fail : term_db.
+Lemma ssubs_esubs U T1 T2 (r : T1 -> term T2) X F (A : formula U T1): rtclosed r ->
+  A[F//X]2⟦r⟧ = A⟦r⟧[F⟦r⟧//X]2.
+Proof. formula_induction A. Qed.
+#[local] Hint Rewrite ssubs_esubs using tauto : term_db.
 
-Lemma ssubs_essubs U1 U2 T (r : U1 -> formula U2 T) X F (A : formula U1 T) :
-  (forall n, sclosed (r n)) -> A[F//X]2⟦r⟧2 = A⟦r⟧2[essubs r F//X]2.
-Proof.
-formula_induction A; rcauto.
-rewrite notin_ssubs; auto.
-now intros H0; rewrite H in H0.
-Qed.
-Hint Rewrite ssubs_essubs using intuition; fail : term_db.
+Lemma subs_essubs U1 U2 T (r : U1 -> formula U2 T) x u A (Hc : rfclosed r) : A[u//x]⟦r⟧2 = A⟦r⟧2[u//x].
+Proof. formula_induction A. Qed.
+#[local] Hint Rewrite subs_essubs using tauto : term_db.
+
+Lemma ssubs_essubs U1 U2 T (r : U1 -> formula U2 T) X F A (Hc : rsclosed r) : A[F//X]2⟦r⟧2 = A⟦r⟧2[F⟦r⟧2//X]2.
+Proof. formula_induction A. Qed.
+#[local] Hint Rewrite ssubs_essubs using tauto : term_db.
 
 
 (* We restrict to [formula nat nat] *)
 (** * Eigen variables *)
 
+Notation "A ↑" := (A⟦⇑⟧) (at level 8, format "A ↑").
+Notation "v ⇓" := (fesubs v) (at level 18, format "v ⇓").
+
+Lemma freevars_fup T (A : formula T nat) : freevars A↑ = freevars A.
+Proof. formula_induction A. Qed.
+#[local] Hint Rewrite freevars_fup : term_db.
+
+Lemma sfreevars_fup T (A : formula T nat) : sfreevars A↑ = sfreevars A.
+Proof. formula_induction A. Qed.
+#[local] Hint Rewrite sfreevars_fup : term_db.
+
+Lemma esubs_fup T v (A : formula T nat) : A↑⟦v⇓⟧ = A.
+Proof. rcauto. Qed.
+#[local] Hint Rewrite esubs_fup : term_db.
+
+Lemma felift_esubs T u r (A : formula T nat) : A↑⟦⇑[u]r⟧ = A⟦r⟧↑.
+Proof. rcauto. Qed.
+#[local] Hint Rewrite felift_esubs : term_db.
+
 Definition sfup T := fun n => @sevar nat T (S n).
 Notation "⇑2" := (sfup nat).
 Notation "A ↑2" := (A⟦⇑2⟧2) (at level 8, format "A ↑2").
+
+Lemma fclosed_sfup : rfclosed ⇑2.
+Proof. reflexivity. Qed.
+Hint Rewrite fclosed_sfup : term_db.
+
+Lemma sclosed_sfup : rsclosed ⇑2.
+Proof. reflexivity. Qed.
+Hint Rewrite sclosed_sfup : term_db.
+
+Lemma fsize_sfup A : fsize A↑2 = fsize A.
+Proof. formula_induction A. Qed.
+#[local] Hint Rewrite fsize_sfup : term_db.
+
+Lemma freevars_sfup A : freevars A↑2 = freevars A.
+Proof. formula_induction A. Qed.
+#[local] Hint Rewrite freevars_sfup : term_db.
+
+Lemma sfreevars_sfup A : sfreevars A↑2 = sfreevars A.
+Proof. formula_induction A. Qed.
+#[local] Hint Rewrite sfreevars_sfup : term_db.
 
 Definition fessubs T (F : formula nat T) := fun n =>
   match n with
@@ -286,6 +402,14 @@ Definition fessubs T (F : formula nat T) := fun n =>
   end.
 Notation "F ⇓2" := (fessubs F) (at level 18, format "F ⇓2").
 
+Lemma fclosed_fessubs T (F : formula nat T) : fclosed F -> rfclosed (F⇓2).
+Proof. now intros Hc [|]. Qed.
+Hint Resolve fclosed_fessubs : term_db.
+
+Lemma sclosed_fessubs T (F : formula nat T) : sclosed F -> rsclosed (F⇓2).
+Proof. now intros Hc [|]. Qed.
+Hint Resolve sclosed_fessubs : term_db.
+
 Definition feslift F r := fun n =>
   match n with
   | 0 => F
@@ -293,13 +417,29 @@ Definition feslift F r := fun n =>
   end.
 Notation "⇑2[ F ] r" := (feslift F r) (at level 25, format "⇑2[ F ] r").
 
+Lemma fclosed_feslift F r : fclosed F -> rfclosed r -> rfclosed (⇑2[F]r).
+Proof. rnow intros ? ? [|]. Qed.
+Hint Resolve fclosed_feslift : term_db.
+
+Lemma sclosed_feslift F r : sclosed F -> rsclosed r -> rsclosed (⇑2[F]r).
+Proof. rnow intros ? ? [|]. Qed.
+Hint Resolve sclosed_feslift : term_db.
+
 Lemma essubs_fup F A : A↑2⟦F⇓2⟧2 = A.
 Proof. rcauto. Qed.
-Hint Rewrite essubs_fup : term_db.
+#[local] Hint Rewrite essubs_fup : term_db.
 
-Lemma felift_essubs F r A : A⟦r⟧2↑2 = A↑2⟦⇑2[F]r⟧2.
+Lemma felift_essubs (r : nat -> formula nat nat) A : A↑⟦fun n => (r n)↑⟧2 = A⟦r⟧2↑.
+Proof. formula_induction A. Qed.
+#[local] Hint Rewrite felift_essubs : term_db.
+
+Lemma feslift_esubs r (A : formula nat nat) : A↑2⟦r⟧ = A⟦r⟧↑2.
+Proof. formula_induction A. Qed.
+#[local] Hint Rewrite feslift_esubs : term_db.
+
+Lemma feslift_essubs F r A : A↑2⟦⇑2[F]r⟧2 = A⟦r⟧2↑2.
 Proof. rcauto. Qed.
-Hint Rewrite felift_essubs : term_db.
+#[local] Hint Rewrite feslift_essubs : term_db.
 
 End Formulas.
 
@@ -330,19 +470,20 @@ Ltac formula_induction A :=
   let lll := fresh "l" in
   let tt := fresh "t" in
   let IHll := fresh "IHl" in
-  induction A as [ n | XX | RR ll | ncon | ucon A ? | bcon A1 ? A2 ?
-                 | qcon xx A | qcon XX A ]; simpl; intros;
-  [ try (apply (f_equal sevar)); try ((rnow idtac) ; fail)
-  | try (apply (f_equal svar)); repeat case_analysis; try ((rnow idtac) ; fail)
+  let IH := fresh "IH" in
+  let IH2 := fresh "IH" in
+  induction A as [ n | XX | RR ll | ncon | ucon A IH | bcon A1 IH A2 IH2
+                 | qcon xx A IH | qcon XX A IH ]; simpl; intros;
+  [ try (apply (f_equal sevar)); try ((rnow idtac); fail)
+  | try (apply (f_equal svar)); repeat case_analysis; try ((rnow idtac); fail)
   | rewrite ? flat_map_concat_map;
     try (apply (f_equal (fvar _)));
     try (induction ll as [ | tt lll IHll ]; simpl; intuition;
          rewrite IHll; f_equal; intuition)
-  | try ((try f_equal); intuition; fail)
+  | try (try f_equal; intuition; fail)
   | try (apply (f_equal (funa _))); intuition
   | try (apply (f_equal2 (fbin _))); intuition
-  | (try apply (f_equal (fqtf _ _))); repeat case_analysis; try (intuition; fail);
-     try (now rcauto)
-  | (try apply (f_equal (sqtf _ _))); repeat case_analysis; try (intuition; fail);
-     try (now rcauto) ];
-  try (now rcauto).
+  | (try apply (f_equal (fqtf _ _))); repeat case_analysis; try (intuition; fail); try now rcauto
+  | (try apply (f_equal (sqtf _ _))); repeat case_analysis; try (intuition; fail); try now rcauto ];
+  try (rewrite ? IH, ? IH2; reflexivity);
+  try now rcauto.
