all.v
@@ -1,0 +1,313 @@
+(* Sequent Calculus for First- and Second-Order Additive Linear Logic *)
+
+From Coq Require Import Wf_nat Lia.
+From Quantifiers Require Import formulas.
+
+Set Implicit Arguments.
+
+
+Parameter vatom : DecType.
+Parameter tatom : Type.
+Parameter satom : DecType.
+Parameter fatom : Type.
+Inductive Ncon := top_con.
+Inductive Bcon := wth_con.
+Inductive Qcon := frl_con.
+
+Notation term := (@term vatom tatom nat).
+Notation tclosed t := (tvars t = nil).
+Notation rtclosed r := (forall n, tclosed (r n)).
+Notation "↑ r" := (felift (evar 0) r) (at level 25, format "↑ r").
+Notation "↑2 r" := (feslift (sevar _ 0) r) (at level 25, format "↑2 r").
+Notation "v ⇓" := (fesubs v) (at level 18, format "v ⇓").
+Notation "F ⇓2" := (fessubs F) (at level 18, format "F ⇓2").
+Notation "A ⟦ r ⟧" := (esubs r A) (at level 8, left associativity, format "A ⟦ r ⟧").
+Notation "A ⟦ r ⟧2" := (essubs r A) (at level 8, left associativity, format "A ⟦ r ⟧2").
+Notation "A [ u // x ]" := (subs x u A) (at level 8, format "A [ u // x ]").
+Notation "A [ F // X ]2" := (ssubs X F A) (at level 8, format "A [ F // X ]2").
+Notation "⇑" := fup.
+Notation "⇑2" := (sfup nat).
+Notation "A ↑" := (A⟦⇑⟧) (at level 8, format "A ↑").
+Notation "A ↑2" := (A⟦⇑2⟧2) (at level 8, format "A ↑2").
+Notation fclosed A := (freevars A = nil).
+Notation rfclosed r := (forall n, fclosed (r n)).
+Notation sclosed A := (sfreevars A = nil).
+Notation rsclosed r := (forall n, sclosed (r n)).
+
+Notation formula := (@formula vatom tatom satom fatom Ncon Nocon Bcon Qcon Qcon nat nat).
+Notation top := (fnul nat nat top_con).
+Notation wth := (fbin wth_con).
+Notation frl := (fqtf frl_con).
+Notation frl2 := (sqtf frl_con).
+Definition evar_nat := (@evar vatom tatom nat).
+Coercion evar_nat : nat >-> term.
+Definition sevar_nat := (@sevar vatom tatom satom fatom Ncon Nocon Bcon Qcon Qcon nat nat).
+Coercion sevar_nat : nat >-> formula.
+Notation sevar := (sevar nat).
+
+#[local] Hint Resolve closed_fesubs : term_db.
+#[local] Hint Resolve closed_felift : term_db.
+#[local] Hint Resolve fclosed_fessubs : term_db.
+#[local] Hint Resolve sclosed_fessubs : term_db.
+#[local] Hint Resolve fclosed_feslift : term_db.
+#[local] Hint Resolve sclosed_feslift : term_db.
+
+#[local] Hint Rewrite (@felift_esubs vatom tatom satom fatom Ncon Nocon Bcon Qcon Qcon) : term_db.
+#[local] Hint Rewrite (@feslift_esubs vatom tatom satom fatom Ncon Nocon Bcon Qcon Qcon) : term_db.
+#[local] Hint Rewrite (@felift_essubs vatom tatom satom fatom Ncon Nocon Bcon Qcon Qcon) : term_db.
+#[local] Hint Rewrite (@feslift_essubs vatom tatom satom fatom Ncon Nocon Bcon Qcon Qcon) : term_db.
+#[local] Hint Rewrite (@esubs_fup vatom tatom satom fatom Ncon Nocon Bcon Qcon Qcon) : term_db.
+#[local] Hint Rewrite (@essubs_fup vatom tatom satom fatom Ncon Nocon Bcon Qcon Qcon) : term_db.
+#[local] Hint Rewrite (@subs_esubs vatom tatom satom fatom Ncon Nocon Bcon Qcon Qcon)
+                        using try tauto; auto with term_db : term_db.
+#[local] Hint Rewrite (@ssubs_esubs vatom tatom satom fatom Ncon Nocon Bcon Qcon Qcon)
+                        using try tauto; auto with term_db : term_db.
+#[local] Hint Rewrite (@subs_essubs vatom tatom satom fatom Ncon Nocon Bcon Qcon Qcon)
+                        using try tauto; auto with term_db : term_db.
+#[local] Hint Rewrite (@ssubs_essubs vatom tatom satom fatom Ncon Nocon Bcon Qcon Qcon)
+                        using try tauto; auto with term_db : term_db.
+#[local] Hint Rewrite (@freevars_fup vatom tatom satom fatom Ncon Nocon Bcon Qcon Qcon) : term_db.
+#[local] Hint Rewrite (@sfreevars_fup vatom tatom satom fatom Ncon Nocon Bcon Qcon Qcon) : term_db.
+
+
+(** * Proofs *)
+
+(** Proofs *)
+(** two-sided sequent calculus for (additive) linear logic with connectives: top, with, forall, forall2 *)
+Inductive prove : formula -> formula -> Type :=
+| ax A : prove A A
+| topr C : prove C top
+| wdgr C A B : prove C A -> prove C B -> prove C (wth A B)
+| wdgll A C B : prove A C -> prove (wth A B) C
+| wdglr A C B : prove A C -> prove (wth B A) C
+| frlr [x C A] : prove (C↑) A↑[0//x] -> prove C (frl x A)
+| frll [x A C] u : tclosed u -> prove A[u//x] C -> prove (frl x A) C
+| frl2r [X C A] : prove (C↑2) A↑2[0//X]2 -> prove C (frl2 X A)
+| frl2l [X A C] F : fclosed F -> sclosed F -> prove A[F//X]2 C -> prove (frl2 X A) C.
+#[local] Hint Constructors prove : term_db.
+
+
+(** height of proofs *)
+Fixpoint psize A B (pi : prove A B) : nat :=
+match pi with
+| ax _ | topr _ => 1
+| wdgr pi1 pi2 => S (max (psize pi1) (psize pi2))
+| wdgll _ pi1 | wdglr _ pi1 => S (psize pi1)
+| frlr pi1 | frll _ _ pi1 | frl2r pi1 | frl2l _ _ _ pi1 => S (psize pi1)
+end.
+
+
+(** proofs with atomic axioms *)
+Fixpoint atomic_proof A B (pi : prove A B) : Prop :=
+match pi with
+| ax A => atomic A
+| topr _ => True
+| wdgr pi1 pi2 => atomic_proof pi1 /\ atomic_proof pi2
+| wdgll _ pi1 | wdglr _ pi1 | frlr pi1 | frll _ _ pi1 | frl2r pi1 | frl2l _ _ _ pi1 => atomic_proof pi1
+end.
+
+
+(** apply [r] in proof [pi] *)
+Theorem pesubs r (Hc : rtclosed r) C A (pi : prove C A) : { pi' : prove C⟦r⟧ A⟦r⟧ & psize pi' = psize pi }.
+Proof.
+induction pi in r, Hc |- *;
+  try (destruct (IHpi r) as [pi' Hs]);
+  try (destruct (IHpi1 r) as [pi1' Hs1]);
+  try (destruct (IHpi2 r) as [pi2' Hs2]); trivial.
+- now exists (ax _).
+- now exists (topr _).
+- exists (wdgr pi1' pi2'). cbn. auto.
+- exists (wdgll _ pi'). cbn. auto.
+- exists (wdglr _ pi'). cbn. auto.
+- clear pi' Hs. destruct (IHpi (↑r)) as [pi' Hs]; [ intuition | ].
+  cbn. rewrite <- Hs. clear Hs.
+  rnow revert pi'.
+  exists (frlr pi'). reflexivity.
+- cbn. rewrite <- Hs. clear Hs.
+  rnow revert pi'.
+  rewrite <- (tvars_tesubs_closed r _ Hc) in e.
+  exists (frll _ e pi'). reflexivity.
+- clear pi' Hs. destruct (IHpi r) as [pi' Hs]; [ intuition | ].
+  cbn. rewrite <- Hs. clear Hs.
+  rnow revert pi'.
+  exists (frl2r pi'). reflexivity.
+- cbn. rewrite <- Hs. clear Hs.
+  rnow revert pi'.
+  rewrite <- (freevars_esubs_closed r) in e by assumption.
+  rewrite <- (sfreevars_esubs r) in e0.
+  exists (frl2l _ e e0 pi'). reflexivity.
+Qed.
+
+Theorem pessubs r (Hcf : rfclosed r) (Hcs : rsclosed r) C A (pi : prove C A) :
+  { pi' : prove C⟦r⟧2 A⟦r⟧2 & psize pi' = psize pi }.
+Proof.
+induction pi in r, Hcf, Hcs |- *;
+  try (destruct (IHpi r) as [pi' Hs]);
+  try (destruct (IHpi1 r) as [pi1' Hs1]);
+  try (destruct (IHpi2 r) as [pi2' Hs2]); trivial.
+- now exists (ax _).
+- now exists (topr _).
+- exists (wdgr pi1' pi2'). cbn. auto.
+- exists (wdgll _ pi'). cbn. auto.
+- exists (wdglr _ pi'). cbn. auto.
+- clear pi' Hs. destruct (IHpi (fun n => (r n)↑)) as [pi' Hs]; rcauto.
+  cbn. rewrite <- Hs. clear Hs.
+  rnow (rnow revert pi').
+  exists (frlr pi'). reflexivity.
+- cbn. rewrite <- Hs. clear Hs.
+  rnow revert pi'.
+  exists (frll _ e pi'). reflexivity.
+- clear pi' Hs. destruct (IHpi (↑2r)) as [pi' Hs]; [ rcauto | rcauto | ].
+  cbn. rewrite <- Hs. clear Hs.
+  rnow revert pi'.
+  exists (frl2r pi'). reflexivity.
+- cbn. rewrite <- Hs. clear Hs.
+  rnow revert pi'.
+  rewrite <- (freevars_essubs_closed _ _ Hcf) in e.
+  rewrite <- (sfreevars_essubs_closed _ _ Hcs) in e0.
+  exists (frl2l _ e e0 pi'). reflexivity.
+Qed.
+
+
+(** * Cut Elimination *)
+
+Theorem cutr A B C : prove A B -> prove B C -> prove A C.
+Proof.
+enough (forall n, forall A B C (pi1 : prove A B) (pi2 : prove B C), n = psize pi1 + psize pi2 -> prove A C) as IH
+  by (intros pi1 pi2; apply (IH _ _ _ _ pi1 pi2 eq_refl)). clear A B C.
+induction n as [n IH0] using lt_wf_rect; intros; subst.
+assert (forall A B C (pi1' : prove A B) (pi2' : prove B C),
+          psize pi1' + psize pi2' < psize pi1 + psize pi2 -> prove A C) as IH
+  by (intros; eapply IH0; [ eassumption | reflexivity ]); clear IH0.
+destruct pi2; intuition.
+- apply wdgr.
+  + apply (IH _ _ _ pi1 pi2_1). cbn. lia.
+  + apply (IH _ _ _ pi1 pi2_2). cbn. lia.
+- enough (forall A D (pi1 : prove A D) A0 B C (pi2 : prove A0 C)
+              (IH : forall A1 B0 C0 (pi1' : prove A1 B0) (pi2' : prove B0 C0),
+                psize pi1' + psize pi2' < psize pi1 + psize (wdgll B pi2) -> prove A1 C0),
+         D = wth A0 B -> prove A C) as IH2
+    by (eapply IH2; [ eassumption | reflexivity ]); clear.
+  intros A D pi1; destruct pi1; intros; inversion H; subst;
+    try (constructor; apply (IH _ _ _ pi1 (wdgll _ pi2)); cbn; lia).
+  + now apply wdgll.
+  + apply (IH _ _ _ pi1_1 pi2). cbn. lia.
+  + apply (frll u); [ assumption | ].
+    apply (IH _ _ _ pi1 (wdgll _ pi2)). cbn. lia.
+  + apply (frl2l F); [ assumption | assumption | ].
+    apply (IH _ _ _ pi1 (wdgll _ pi2)). cbn. lia.
+- enough (forall A D (pi1 : prove A D) A0 B C (pi2 : prove A0 C)
+              (IH : forall A1 B0 C0 (pi1' : prove A1 B0) (pi2' : prove B0 C0),
+                 psize pi1' + psize pi2' < psize pi1 + psize (wdglr B pi2) -> prove A1 C0),
+         D = wth B A0 -> prove A C) as IH2
+    by (eapply IH2 ; [ eassumption | reflexivity ]); clear.
+  intros A D pi1; destruct pi1; intros; inversion H; subst;
+    try (constructor; apply (IH _ _ _ pi1 (wdglr _ pi2)); cbn; lia).
+  + now apply wdglr.
+  + apply (IH _ _ _ pi1_2 pi2). cbn. lia.
+  + apply (frll u); [ assumption | ].
+    apply (IH _ _ _ pi1 (wdglr _ pi2)). cbn. lia.
+  + apply (frl2l F); [ assumption | assumption | ].
+    apply (IH _ _ _ pi1 (wdglr _ pi2)). cbn. lia.
+- destruct (pesubs ⇑ closed_fup pi1) as [pi1' Hs].
+  apply frlr, (IH _ _ _ pi1' pi2). cbn. lia.
+- enough (forall A D (pi1 : prove A D) x A0 C u e (pi2 : prove A0[u//x] C)
+              (IH : forall A1 B C0 (pi1' : prove A1 B) (pi2' : prove B C0),
+                 psize pi1' + psize pi2' < psize pi1 + psize (frll u e pi2) -> prove A1 C0),
+         D = frl x A0 -> prove A C) as IH2
+    by (eapply IH2; [ eassumption | reflexivity ]); clear.
+  intros A D pi1; destruct pi1; intros; inversion H; subst;
+    try (constructor; apply (IH _ _ _ pi1 (frll _ e pi2)); cbn; lia).
+  + now apply (frll u).
+  + destruct (pesubs (u⇓) (closed_fesubs _ e) pi1) as [pi1' Hs].
+    simpl in IH. rewrite <- Hs in IH. clear Hs.
+    rnow revert pi1' IH.
+    apply (IH _ _ _ pi1' pi2). lia.
+  + apply (frll u); [ assumption | ].
+    apply (IH _ _ _ pi1 (frll _ e0 pi2)). cbn. lia.
+  + apply (frl2l F); [ assumption | assumption | ].
+    apply (IH _ _ _ pi1 (frll _ e1 pi2)). cbn. lia.
+- destruct (pessubs ⇑2 fclosed_sfup sclosed_sfup pi1) as [pi1' Hs].
+  apply frl2r, (IH _ _ _ pi1' pi2). cbn. lia.
+- enough (forall A D (pi1 : prove A D) X A0 C F e e' (pi2 : prove A0[F//X]2 C)
+              (IH : forall A1 B C0 (pi1' : prove A1 B) (pi2' : prove B C0),
+                 psize pi1' + psize pi2' < psize pi1 + psize (frl2l F e e' pi2) -> prove A1 C0),
+         D = frl2 X A0 -> prove A C) as IH2
+    by (eapply IH2; [ eassumption | reflexivity ]); clear.
+  intros A D pi1; destruct pi1; intros; inversion H; subst;
+    try (constructor; apply (IH _ _ _ pi1 (frl2l _ e e' pi2)); cbn; lia).
+  + now apply (frl2l F).
+  + apply (frll u); [ assumption | ].
+    apply (IH _ _ _ pi1 (frl2l _ e0 e' pi2)). cbn. lia.
+  + destruct (pessubs (F⇓2) (fclosed_fessubs _ e) (sclosed_fessubs _ e') pi1) as [pi1' Hs].
+    simpl in IH. rewrite <- Hs in IH. clear Hs.
+    rnow revert pi1' IH.
+    apply (IH _ _ _ pi1' pi2). lia.
+  + apply (frl2l F); [ assumption | assumption | ].
+    apply (IH _ _ _ pi1 (frl2l _ e1 e' pi2)). cbn. lia.
+Qed.
+
+
+(** * Axiom expansion *)
+
+Lemma ax_gen_size A : { pi : prove A A | atomic_proof pi & psize pi < 2 * fsize A }.
+Proof.
+enough (Hn : forall n A, fsize A = n -> { pi : prove A A | atomic_proof pi & psize pi < 2 * fsize A })
+  by (eapply Hn; reflexivity).
+clear A. intro n. induction n as [n IH] using lt_wf_rect. intros A <-.
+destruct A; [ | | | destruct n | destruct n | destruct b | destruct q | destruct q ].
+- exists (ax _); [ constructor | cbn; lia ].
+- exists (ax _); [ constructor | cbn; lia ].
+- exists (ax _); [ constructor | cbn; lia ].
+- exists (topr _); [ constructor | cbn; lia ].
+- assert (fsize A1 < fsize (wth A1 A2)) as Hs1 by (cbn; lia).
+  destruct (IH _ Hs1 _ eq_refl) as [pi1 Hat1 Hsize1].
+  assert (fsize A2 < fsize (wth A1 A2)) as Hs2 by (cbn; lia).
+  destruct (IH _ Hs2 _ eq_refl) as [pi2 Hat2 Hsize2].
+  exists (wdgr (wdgll A2 pi1) (wdglr A1 pi2)); [ constructor; assumption | cbn; lia ].
+- assert (fsize (A↑[0//c]) < fsize (frl c A)) as Hs.
+  { rewrite fsize_subs, fsize_esubs. cbn. lia. }
+  destruct (IH _ Hs _ eq_refl) as [pi Hat Hsize].
+  exists (frlr (frll 0 eq_refl pi : prove ((frl c A)↑) _)); [ assumption | cbn in *; lia ].
+- assert (fsize (A↑2[0//c]2) < fsize (frl2 c A)) as Hs.
+  { rewrite fsize_ssubs_atomic, fsize_sfup by constructor. cbn. lia. }
+  destruct (IH _ Hs _ eq_refl) as [pi Hat Hsize].
+  exists (frl2r (frl2l 0 eq_refl eq_refl pi : prove ((frl2 c A)↑2) _)); [ assumption | cbn in *; lia ].
+Qed.
+
+Lemma ax_gen A : prove A A.
+Proof. apply (ax_gen_size A). Qed.
+
+Lemma ax_exp A B : prove A B -> { pi : prove A B | atomic_proof pi }.
+Proof.
+intros pi0. induction pi0.
+- destruct (ax_gen_size A) as [pi Hat _].
+  exists pi. exact Hat.
+- exists (topr _). constructor.
+- destruct IHpi0_1 as [pi1 Hat1], IHpi0_2 as [pi2 Hat2].
+  exists (wdgr pi1 pi2). constructor; assumption.
+- destruct IHpi0 as [pi Hat].
+  exists (wdgll B pi). assumption.
+- destruct IHpi0 as [pi Hat].
+  exists (wdglr B pi). assumption.
+- destruct IHpi0 as [pi Hat].
+  exists (frlr pi). assumption.
+- destruct IHpi0 as [pi Hat].
+  exists (frll _ e pi). assumption.
+- destruct IHpi0 as [pi Hat].
+  exists (frl2r pi). assumption.
+- destruct IHpi0 as [pi Hat].
+  exists (frl2l _ e e0 pi). assumption.
+Qed.
+
+
+(** * Hilbert style properties *)
+
+Lemma frl_elim A u x : tclosed u -> prove (frl x A) A[u//x].
+Proof. intros Hc. apply (frll u), ax_gen. exact Hc. Qed.
+
+Lemma frl_wth A B x : prove (frl x (wth A B)) (wth (frl x A) (frl x B)).
+Proof. repeat constructor; cbn; apply (frll 0); cbn; constructor; apply ax_gen. Qed.
+
+Lemma frl_nfree A x : ~ In x (freevars A) -> prove A (frl x A).
+Proof. intros Hnf. apply frlr. rewrite nfree_subs; [ apply ax_gen | rcauto ]. Qed.
