all2.v
@@ -125,30 +125,29 @@ match A with
 end.
 Notation closed A := (freevars A = nil).
 
-Lemma closed_nofreevars : forall A X, closed A -> ~ In X (freevars A).
-Proof. intros A X Hc Hin ; now rewrite Hc in Hin. Qed.
+Lemma closed_nofreevars A X : closed A -> ~ In X (freevars A).
+Proof. intros Hc Hin. rewrite Hc in Hin. destruct Hin. Qed.
 
-Lemma freevars_fup : forall k A, freevars (fup k A) = freevars A.
+Lemma freevars_fup k A : freevars (fup k A) = freevars A.
 Proof. formula_induction A. Qed.
 #[local] Hint Rewrite freevars_fup : term_db.
 
-Lemma freevars_nsubs : forall n F, closed F -> forall A,
-  freevars (nsubs n F A) = freevars A.
+Lemma freevars_nsubs n F (Hc : closed F) A : freevars (nsubs n F A) = freevars A.
 Proof. formula_induction A. Qed.
 #[local] Hint Rewrite freevars_nsubs using assumption : term_db.
 
-Lemma nfree_subs : forall X F A, ~ In X (freevars A) -> subs X F A = A.
-Proof. formula_induction A ; rcauto; now f_equal. Qed.
-#[local] Hint Rewrite nfree_subs using try (intuition ; fail) ;
-                              (try apply closed_nofreevars) ; intuition ; fail : term_db.
+Lemma nfree_subs X F A : ~ In X (freevars A) -> subs X F A = A.
+Proof. formula_induction A. Qed.
+#[local] Hint Rewrite nfree_subs using try tauto;
+                                       try apply closed_nofreevars; tauto : term_db.
 
-Lemma nsubs_subs_com : forall X F n G, ~ In X (freevars G) -> forall A,
+Lemma nsubs_subs_com X F n G (Hin : ~ In X (freevars G)) A :
   nsubs n G (subs X F A) = subs X (nsubs n G F) (nsubs n G A).
-Proof. now formula_induction A ; rcauto ; f_equal. Qed.
-#[local] Hint Rewrite nsubs_subs_com using try (intuition ; fail) ;
-                                  (try apply closed_nofreevars) ; intuition ; fail : term_db.
+Proof. formula_induction A. Qed.
+#[local] Hint Rewrite nsubs_subs_com using try tauto;
+                                           try apply closed_nofreevars; tauto : term_db.
 
-Lemma nsubs_z_fup : forall F A, nsubs 0 F (fupz A) = A.
+Lemma nsubs_z_fup F A : nsubs 0 F (fupz A) = A.
 Proof. formula_induction A. Qed.
 #[local] Hint Rewrite nsubs_z_fup : term_db.
 
@@ -184,107 +183,104 @@ end.
 (** substitutes [cterm] [u] for index [n] in proof [pi] and decreases indexes above [n] *)
 Theorem psubs k F (Hc : closed F) {C A} (pi : prove C A) :
   { pi' : prove (nsubs k F C) (nsubs k F A) | psize pi' = psize pi }.
-Proof with autorewrite with term_db.
-revert k F Hc ; induction pi ; intros k F' Hc ;
-  try (destruct (IHpi k F' Hc) as [pi' Hs]) ;
-  try (destruct (IHpi1 k F' Hc) as [pi1' Hs1]) ;
+Proof.
+revert k F Hc; induction pi; intros k F' Hc;
+  try (destruct (IHpi k F' Hc) as [pi' Hs]);
+  try (destruct (IHpi1 k F' Hc) as [pi1' Hs1]);
   try (destruct (IHpi2 k F' Hc) as [pi2' Hs2]).
 - now exists (ax _).
 - now exists (topr _).
-- exists (wdgr pi1' pi2') ; simpl ; auto.
-- exists (wdgll _ pi') ; simpl ; auto.
-- exists (wdglr _ pi') ; simpl ; auto.
+- exists (wdgr pi1' pi2'). cbn. auto.
+- exists (wdgll _ pi'). cbn. auto.
+- exists (wdglr _ pi'). cbn. auto.
 - clear pi' Hs.
   rewrite <- (freevars_fup 0) in Hc.
   destruct (IHpi (S k) _ Hc) as [pi' Hs].
-  simpl ; rewrite <- Hs ; clear Hs.
-  revert pi'...
-  intros pi' ; exists (frlr pi') ; reflexivity.
-- simpl ; rewrite <- Hs ; clear Hs.
-  revert pi'...
+  cbn. rewrite <- Hs. clear Hs.
+  rnow revert pi'.
+  exists (frlr pi'). reflexivity.
+- cbn. rewrite <- Hs. clear Hs.
+  rnow revert pi'.
   rewrite <- (freevars_nsubs k F' Hc) in e.
-  intros pi' ; exists (frll _ e pi') ; reflexivity.
+  exists (frll _ e pi'). reflexivity.
 Qed.
 
 (** lift indexes above [k] in proof [pi] *)
-Theorem pup k {C A} (pi : prove C A) :
-  { pi' : prove (fup k C) (fup k A) | psize pi' = psize pi }.
-Proof with autorewrite with term_db.
-revert k ; induction pi ; intros k ;
+Theorem pup k {C A} (pi : prove C A) : { pi' : prove (fup k C) (fup k A) | psize pi' = psize pi }.
+Proof.
+induction pi in k |- *;
   try (destruct (IHpi k) as [pi' Hs]) ;
   try (destruct (IHpi1 k) as [pi1' Hs1]) ;
   try (destruct (IHpi2 k) as [pi2' Hs2]).
 - now exists (ax _).
 - now exists (topr _).
-- exists (wdgr pi1' pi2') ; simpl ; auto.
-- exists (wdgll _ pi') ; simpl ; auto.
-- exists (wdglr _ pi') ; simpl ; auto.
+- exists (wdgr pi1' pi2'). cbn. auto.
+- exists (wdgll _ pi'). cbn. auto.
+- exists (wdglr _ pi'). cbn. auto.
 - clear pi' Hs.
   destruct (IHpi (S k)) as [pi' Hs].
-  simpl ; rewrite <- Hs ; clear Hs.
+  cbn. rewrite <- Hs. clear Hs.
   revert pi'.
-  change (dvar 0) with (fup (S k) (dvar 0))...
-  intros pi' ; exists (frlr pi') ; reflexivity.
-- simpl ; rewrite <- Hs ; clear Hs.
-  revert pi'...
+  rnow change (dvar 0) with (fup (S k) (dvar 0)).
+  exists (frlr pi'). reflexivity.
+- cbn. rewrite <- Hs. clear Hs.
+  rnow revert pi'.
   rewrite <- (freevars_fup k) in e.
-  intros pi' ; exists (frll _ e pi') ; reflexivity.
+  exists (frll _ e pi'). reflexivity.
 Qed.
 
 
 
 (** * Cut Elimination *)
 
-Theorem cutr : forall A B C, prove A B -> prove B C -> prove A C.
-Proof with try lia.
-enough (H : forall n, forall A B C (pi1 : prove A B) (pi2 : prove B C),
-              n = psize pi1 + psize pi2 -> prove A C)
-  by (intros A B C pi1 pi2 ; apply (H _ _ _ _ pi1 pi2 eq_refl)).
+Theorem cutr A B C : prove A B -> prove B C -> prove A C.
+Proof.
+enough (forall n, forall A B C (pi1 : prove A B) (pi2 : prove B C),
+              n = psize pi1 + psize pi2 -> prove A C) as H
+  by (intros pi1 pi2 ; apply (H _ _ _ _ pi1 pi2 eq_refl)). clear A B C.
 induction n as [n IH0] using (well_founded_induction_type lt_wf) ; intros ; subst.
-assert (IH : forall A B C (pi1' : prove A B) (pi2' : prove B C),
-               psize pi1' + psize pi2' < psize pi1 + psize pi2 -> prove A C)
-  by (intros ; eapply IH0 ; eauto) ; clear IH0.
-destruct pi2 ; intuition.
+assert (forall A B C (pi1' : prove A B) (pi2' : prove B C),
+               psize pi1' + psize pi2' < psize pi1 + psize pi2 -> prove A C) as IH
+  by (intros; eapply IH0; eauto); clear IH0.
+destruct pi2; intuition.
 - apply wdgr.
-  + apply (IH _ _ _ pi1 pi2_1) ; simpl...
-  + apply (IH _ _ _ pi1 pi2_2) ; simpl...
+  + apply (IH _ _ _ pi1 pi2_1). cbn. lia.
+  + apply (IH _ _ _ pi1 pi2_2). cbn. lia.
 - enough (forall A D (pi1 : prove A D) A0 B C (pi2 : prove A0 C)
             (IH : forall A1 B0 C0 (pi1' : prove A1 B0) (pi2' : prove B0 C0),
                    psize pi1' + psize pi2' < psize pi1 + psize (wdgll B pi2) -> prove A1 C0),
          D = wdg A0 B -> prove A C)
-    as IH2 by refine (IH2 _ _ _ _ _ _ _ IH eq_refl) ; clear.
-  intros A D pi1 ; destruct pi1 ; intros ; inversion H ; subst ; intuition ;
-    try (constructor ; apply (IH _ _ _ pi1 (wdgll _ pi2)) ; simpl ; lia).
-  + apply (IH _ _ _ pi1_1 pi2) ; simpl...
+    as IH2 by refine (IH2 _ _ _ _ _ _ _ IH eq_refl); clear.
+  intros A D pi1; destruct pi1; intros; inversion H; subst; intuition;
+    try (constructor ; apply (IH _ _ _ pi1 (wdgll _ pi2)); cbn; lia).
+  + apply (IH _ _ _ pi1_1 pi2). cbn. lia.
   + apply (frll F e).
-    apply (IH _ _ _ pi1 (wdgll _ pi2)) ; simpl...
+    apply (IH _ _ _ pi1 (wdgll _ pi2)). cbn. lia.
 - enough (forall A D (pi1 : prove A D) A0 B C (pi2 : prove A0 C)
             (IH : forall A1 B0 C0 (pi1' : prove A1 B0) (pi2' : prove B0 C0),
                 psize pi1' + psize pi2' < psize pi1 + psize (wdglr B pi2) -> prove A1 C0),
          D = wdg B A0 -> prove A C)
     as IH2 by refine (IH2 _ _ _ _ _ _ _ IH eq_refl) ; clear.
-  intros A D pi1 ; destruct pi1 ; intros ; inversion H ; subst ; intuition ;
-    try (constructor ; apply (IH _ _ _ pi1 (wdglr _ pi2)) ; simpl ; lia).
-  + apply (IH _ _ _ pi1_2 pi2) ; simpl...
+  intros A D pi1; destruct pi1; intros; inversion H; subst; intuition;
+    try (constructor; apply (IH _ _ _ pi1 (wdglr _ pi2)); cbn; lia).
+  + apply (IH _ _ _ pi1_2 pi2). cbn. lia.
   + apply (frll F e).
-    apply (IH _ _ _ pi1 (wdglr _ pi2)) ; simpl...
+    apply (IH _ _ _ pi1 (wdglr _ pi2)). cbn. lia.
 - destruct (pup 0 pi1) as [pi1' Hs].
-  apply frlr.
-  apply (IH _ _ _ pi1' pi2) ; simpl...
+  apply frlr, (IH _ _ _ pi1' pi2). cbn. lia.
 - enough (forall A D (pi1 : prove A D) X A0 C F e (pi2 : prove (subs X F A0) C)
             (IH : forall A1 B C0 (pi1' : prove A1 B) (pi2' : prove B C0),
                    psize pi1' + psize pi2' < psize pi1 + psize (frll F e pi2) -> prove A1 C0),
          D = frl X A0 -> prove A C)
-    as IH2 by refine (IH2 _ _ _ _ _ _ _ _ _ IH eq_refl) ; clear.
-  intros A D pi1 ; destruct pi1 ; intros ; inversion H ; subst ;
-    try (constructor ; apply (IH _ _ _ pi1 (frll _ e pi2)) ; simpl ; lia).
-  + apply (frll F e) ; assumption.
+    as IH2 by refine (IH2 _ _ _ _ _ _ _ _ _ IH eq_refl); clear.
+  intros A D pi1; destruct pi1; intros; inversion H; subst;
+    try (constructor ; apply (IH _ _ _ pi1 (frll _ e pi2)); cbn; lia).
+  + apply (frll F e). assumption.
   + destruct (psubs 0 F e pi1) as [pi1' Hs].
-    simpl in IH ; rewrite <- Hs in IH ; clear Hs.
-    revert pi1' IH ; autorewrite with term_db.
-    intros pi1' IH ; apply (IH _ _ _ pi1' pi2) ; simpl...
-  + apply (frll F e).
-    apply (IH _ _ _ pi1 (frll F0 e0 pi2)) ; simpl...
+    simpl in IH. rewrite <- Hs in IH. clear Hs.
+    revert pi1' IH. autorewrite with term_db. intros pi1' IH.
+    apply (IH _ _ _ pi1' pi2). cbn. lia.
+  + apply (frll F e), (IH _ _ _ pi1 (frll F0 e0 pi2)). cbn. lia.
 Qed.
 
 
@@ -317,15 +313,14 @@ Qed.
 (** Axiom expansion *)
 Lemma ax_exp : forall A, prove A A.
 Proof.
-enough (Hn : forall n A, fsize A = n -> prove A A)
-  by (intros A ; refine (Hn _ _ eq_refl)).
-induction n as [n IH] using (well_founded_induction_type lt_wf) ; intros ; subst.
+enough (Hn : forall n A, fsize A = n -> prove A A) by (intros A; refine (Hn _ _ eq_refl)).
+induction n as [n IH] using (well_founded_induction_type lt_wf); intros; subst.
 destruct A.
 - apply ax.
 - apply ax.
 - apply ax.
 - apply topr.
-- apply wdgr ; [ apply wdgll | apply wdglr ] ; refine (IH _ _ _ eq_refl) ; simpl ; lia.
+- apply wdgr; [ apply wdgll | apply wdglr ]; refine (IH _ _ _ eq_refl); cbn; lia.
 - apply frlr.
-  simpl ; apply (frll (dvar 0) eq_refl) ; auto with term_db.
+  cbn. apply (frll (dvar 0) eq_refl). constructor.
 Qed.
