foterms_ar.v
@@ -126,7 +126,6 @@ end.
 Notation "x ∈ t" := (In x (tvars t)) (at level 30).
 Notation "x ∉ t" := (~ In x (tvars t)) (at level 30).
 Notation closed t := (tvars t = nil).
-Notation fclosed r := (forall n, closed (r n)).
 
 Lemma closed_notvars t x : closed t -> x ∉ t.
 Proof. intros Hc Hin. rewrite Hc in Hin. destruct Hin. Qed.
@@ -164,7 +163,7 @@ Variable T1 T2 : Type.
 Variable r : T1 -> term T2 0.
 
 Notation closed t := (tvars t = nil).
-Notation fclosed := (forall n, closed (r n)).
+Notation rclosed := (forall n, closed (r n)).
 Notation "t [ u // x ]" := (tsubs x u t) (at level 8, format "t [ u // x ]").
 
 Hint Rewrite notin_tsubs using try easy;
@@ -173,11 +172,11 @@ Hint Rewrite notin_tsubs using try easy;
 
 (** * Additional results with variable eigen type *)
 
-Lemma tvars_tesubs_fclosed k (t : term T1 k) : fclosed -> tvars t⟦r⟧ = tvars t.
+Lemma tvars_tesubs_closed k (t : term T1 k) : rclosed -> tvars t⟦r⟧ = tvars t.
 Proof. term_induction t. Qed.
-Hint Rewrite tvars_tesubs_fclosed using intuition; fail : term_db.
+Hint Rewrite tvars_tesubs_closed using intuition; fail : term_db.
 
-Lemma tsubs_tesubs x u k (t : term T1 k) : fclosed -> t[u//x]⟦r⟧ = t⟦r⟧[u⟦r⟧//x].
+Lemma tsubs_tesubs x u k (t : term T1 k) : rclosed -> t[u//x]⟦r⟧ = t⟦r⟧[u⟦r⟧//x].
 Proof. term_induction t. Qed.
 Hint Rewrite tsubs_tesubs using intuition; fail : term_db.
 
@@ -187,7 +186,7 @@ End Two_Eigen_Types.
 (* We restrict to [term nat] *)
 Section Eigen_nat.
 
-Hint Rewrite tvars_tesubs_fclosed using intuition; fail : term_db.
+Hint Rewrite tvars_tesubs_closed using intuition; fail : term_db.
 
 Notation term := (term nat).
 Notation tvar := (tvar nat).
@@ -195,15 +194,15 @@ Notation "t [ u // x ]" := (tsubs x u t) (at level 8, format "t [ u // x ]").
 Notation "x ∈ t" := (In x (tvars t)) (at level 30).
 Notation "x ∉ t" := (~ In x (tvars t)) (at level 30).
 Notation closed t := (tvars t = nil).
-Notation fclosed r := (forall n, closed (r n)).
+Notation rclosed r := (forall n, closed (r n)).
 
 Definition fup := fun n => evar (S n).
 Notation "⇑" := fup.
 Notation "t ↑" := (t⟦⇑⟧) (at level 8, format "t ↑").
 
-Lemma fclosed_fup : fclosed ⇑.
+Lemma closed_fup : rclosed ⇑.
 Proof. reflexivity. Qed.
-Hint Rewrite fclosed_fup : term_db.
+Hint Rewrite closed_fup : term_db.
 
 Lemma tvars_fup k (t : term k) : tvars t↑ = tvars t.
 Proof. rcauto. Qed.
@@ -216,9 +215,9 @@ Definition fesubs v := fun n =>
   end.
 Notation "v ⇓" := (fesubs v) (at level 18, format "v ⇓").
 
-Lemma fclosed_fesubs v : closed v -> fclosed (v⇓).
+Lemma closed_fesubs v : closed v -> rclosed (v⇓).
 Proof. now intros Hc [|]. Qed.
-Hint Resolve fclosed_fesubs : term_db.
+Hint Resolve closed_fesubs : term_db.
 
 Lemma fesubs_fup v : ⇑ ;; v⇓ ~ evar.
 Proof. intro. reflexivity. Qed.
@@ -235,9 +234,9 @@ Definition felift u (r : _ -> term 0) := fun n =>
   end.
 Notation "⇑[ u ] r" := (felift u r) (at level 25, format "⇑[ u ] r").
 
-Lemma fclosed_felift u r : closed u -> fclosed r -> fclosed (⇑[u]r).
+Lemma closed_felift u r : closed u -> rclosed r -> rclosed (⇑[u]r).
 Proof. rnow intros ? ? [|]. Qed.
-Hint Resolve fclosed_felift : term_db.
+Hint Resolve closed_felift : term_db.
 
 Lemma felift_comp u r : r ;; ⇑ ~ ⇑ ;; ⇑[u]r.
 Proof. intro. reflexivity. Qed.
