foterms_std.v
@@ -11,15 +11,15 @@ Context { vatom : DecType } { tatom : Type }.
 
 Notation "r ;; s" := (fecomp r s) (at level 20, format "r  ;;  s").
 Notation closed t := (tvars t = nil).
-Notation fclosed r := (forall n, closed (r n)).
+Notation rclosed r := (forall n, closed (r n)).
 
 (* Function allowing to embed [term Empty_set] into any [term T]
      through identity embedding by using [tesubs (r_empty T)] *)
 Definition r_empty T : Empty_set -> @term vatom tatom T := fun z => match z with end.
 
-Lemma fclosed_r_empty T : fclosed (r_empty T).
+Lemma closed_r_empty T : rclosed (r_empty T).
 Proof. intros []. Qed.
-Hint Resolve fclosed_r_empty : term_db.
+Hint Resolve closed_r_empty : term_db.
 
 Lemma fecomp_r_empty T1 T2 s : r_empty T1 ;; s ~ r_empty T2.
 Proof. intros []. Qed.
