nj1.v
@@ -17,7 +17,7 @@ Arguments tvar {_} {_} {T} _.
 
 Notation term := (@term vatom tatom nat).
 Notation closed t := (tvars t = nil).
-Notation fclosed r := (forall n, closed (r n)).
+Notation rclosed r := (forall n, closed (r n)).
 Notation "↑ r" := (felift (evar 0) r) (at level 25, format "↑ r").
 Notation "v ⇓" := (fesubs v) (at level 18, format "v ⇓").
 Notation "A ⟦ r ⟧" := (esubs r A) (at level 8, left associativity, format "A ⟦ r ⟧").
@@ -30,18 +30,18 @@ Notation formula := (@formula vatom tatom fatom Nocon Nocon Icon Qcon nat).
 
 Hint Rewrite (@fsize_esubs vatom tatom fatom Nocon Nocon Icon Qcon) : term_db.
 Hint Rewrite (@fsize_subs vatom tatom fatom Nocon Nocon Icon Qcon nat) : term_db.
-Hint Rewrite (@tvars_tesubs_fclosed vatom tatom) using intuition; fail : term_db.
-Hint Rewrite (@freevars_esubs_fclosed vatom tatom fatom Nocon Nocon Icon Qcon nat)
+Hint Rewrite (@tvars_tesubs_closed vatom tatom) using intuition; fail : term_db.
+Hint Rewrite (@freevars_esubs_closed vatom tatom fatom Nocon Nocon Icon Qcon nat)
                  using intuition; fail : term_db.
 Hint Rewrite (@subs_esubs_notegen vatom tatom fatom Nocon Nocon Icon Qcon nat)
                          using try (intuition; fail);
-                             (try apply no_ecapture_not_egenerated); try (intuition; fail);
-                             (try apply fclosed_no_ecapture); intuition; fail : term_db.
-Hint Rewrite <- (@felift_esubs vatom tatom fatom Nocon Nocon Icon Qcon) : term_db.
+                             try apply no_ecapture_not_egenerated; try (intuition; fail);
+                             try apply closed_no_ecapture; intuition; fail : term_db.
+Hint Rewrite (@felift_esubs vatom tatom fatom Nocon Nocon Icon Qcon) : term_db.
 Hint Rewrite (@esubs_fup vatom tatom fatom Nocon Nocon Icon Qcon) : term_db.
 
-Hint Resolve fclosed_felift : term_db.
-Hint Resolve fclosed_fesubs : term_db.
+Hint Resolve closed_felift : term_db.
+Hint Resolve closed_fesubs : term_db.
 
 
 (** Proofs *)
@@ -122,13 +122,13 @@ Proof. now apply rnprove_mutrect; intros; try (econstructor; eassumption). Qed.
 (** * Normalization *)
 
 (** apply [r] in normal form *)
-Theorem rnpesubs r (Hc : fclosed r) {l A} :
+Theorem rnpesubs r (Hc : rclosed r) {l A} :
    (nprove l A -> nprove (map (esubs r) l) A⟦r⟧)
  * (rprove l A -> rprove (map (esubs r) l) A⟦r⟧).
 Proof.
 revert l A.
-enough ((forall l A, nprove l A -> forall r, fclosed r -> nprove (map (esubs r) l) A⟦r⟧)
-      * (forall l A, rprove l A -> forall r, fclosed r -> rprove (map (esubs r) l) A⟦r⟧))
+enough ((forall l A, nprove l A -> forall r, rclosed r -> nprove (map (esubs r) l) A⟦r⟧)
+      * (forall l A, rprove l A -> forall r, rclosed r -> rprove (map (esubs r) l) A⟦r⟧))
   as He by (split; intros; apply He; assumption).
 clear r Hc; apply rnprove_mutrect; intros; (try simpl in X);
   (try assert (IH1 := X r H)); (try assert (IH2 := X0 r H));
@@ -137,16 +137,15 @@ clear r Hc; apply rnprove_mutrect; intros; (try simpl in X);
 - rcauto; rnow apply nfrle.
 - specialize X with (↑r0).
   revert X; rcauto.
-  rewrite map_map, <- (map_ext _ _ (felift_esubs (evar 0) _)), <- map_map in X; intuition.
+  rewrite map_map, (map_ext _ _ (felift_esubs (evar 0) _)), <- map_map in X. intuition.
 - specialize X with r0.
   rnow apply (rexsi (tesubs r0 u)).
 - specialize X0 with (↑r0); simpl in X0.
-  rewrite map_map, <- (map_ext _ _ (felift_esubs (evar 0) _)), <- map_map in X0.
+  rewrite map_map, (map_ext _ _ (felift_esubs (evar 0) _)), <- map_map in X0.
   rnow eapply rexse.
 Qed.
 
-Lemma rpsubsz_r {l A x u} : closed u ->
-  rprove l⇈ A↑[evar 0//x] -> rprove l (subs x u A).
+Lemma rpsubsz_r {l A x u} : closed u -> rprove l⇈ A↑[evar 0//x] -> rprove l (subs x u A).
 Proof.
 intros Hc pi.
 apply (rnpesubs (u⇓)) in pi; [ | intuition ].
@@ -154,8 +153,7 @@ rnow simpl in pi then simpl in pi.
 now rewrite map_map, (map_ext _ _ (esubs_fup _)), map_id in pi.
 Qed.
 
-Lemma rpsubsz_l {l A x u C} : closed u ->
-  rprove (A↑[evar 0//x] :: l⇈) C↑ -> rprove (subs x u A :: l) C.
+Lemma rpsubsz_l {l A x u C} : closed u -> rprove (A↑[evar 0//x] :: l⇈) C↑ -> rprove (subs x u A :: l) C.
 Proof.
 intros Hc pi.
 apply (rnpesubs (u⇓)) in pi; [ | intuition ].
@@ -224,7 +222,7 @@ remember (exs x A) as A'; revert A x HeqA'; induction pi;
     eapply rweakening; [ | reflexivity ].
     apply (rnpesubs (↑⇑)) in pi2; intuition.
     rnow simpl in pi2 then simpl in pi2.
-    now rewrite map_map, <- (map_ext _ _ (felift_esubs (evar 0) _)), <- map_map in pi2.
+    now rewrite map_map, (map_ext _ _ (felift_esubs (evar 0) _)), <- map_map in pi2.
 Qed.
 
 Lemma substitution : forall n m A, fsize A = n ->
@@ -294,7 +292,7 @@ apply (lt_wf_double_rect (fun n m =>
 - eapply rexsi; eauto.
   refine (snd (IHm _ _ _ _) _ _ _ pi2 _ _); auto; lia.
 - rewrite <- (app_nil_l _) in pi1.
-  assert (pi1' := snd rweakening _ _ (snd (rnpesubs ⇑ fclosed_fup) pi1)
+  assert (pi1' := snd rweakening _ _ (snd (rnpesubs ⇑ closed_fup) pi1)
                   (A0↑[evar 0//x] :: nil) nil _ eq_refl) ; simpl in pi1'.
   rewrite map_app in pi1' ; rewrite app_comm_cons in pi1'.
   revert pi2 pi1' Hpi; rewrite ? map_app; simpl; rewrite app_comm_cons;
