nj1_frl.v
@@ -17,7 +17,7 @@ Arguments tvar {_} {_} {T} _.
 
 Notation term := (@term vatom tatom nat).
 Notation closed t := (tvars t = nil).
-Notation fclosed r := (forall n, closed (r n)).
+Notation rclosed r := (forall n, closed (r n)).
 Notation "↑ r" := (felift (evar 0) r) (at level 25, format "↑ r").
 Notation "v ⇓" := (fesubs v) (at level 18, format "v ⇓").
 Notation "A ⟦ r ⟧" := (esubs r A) (at level 8, left associativity, format "A ⟦ r ⟧").
@@ -33,14 +33,14 @@ Notation formula := (@formula vatom tatom fatom Nocon Nocon Icon FQcon nat).
 
 Hint Rewrite (@fsize_esubs vatom tatom fatom Nocon Nocon Icon FQcon) : term_db.
 Hint Rewrite (@fsize_subs vatom tatom fatom Nocon Nocon Icon FQcon nat) : term_db.
-Hint Rewrite (@tvars_tesubs_fclosed vatom tatom) using intuition; fail : term_db.
+Hint Rewrite (@tvars_tesubs_closed vatom tatom) using intuition; fail : term_db.
 Hint Rewrite (@subs_esubs vatom tatom fatom Nocon Nocon Icon FQcon nat)
                          using intuition; fail : term_db.
-Hint Rewrite <- (@felift_esubs vatom tatom fatom Nocon Nocon Icon FQcon) : term_db.
+Hint Rewrite (@felift_esubs vatom tatom fatom Nocon Nocon Icon FQcon) : term_db.
 Hint Rewrite (@esubs_fup vatom tatom fatom Nocon Nocon Icon FQcon) : term_db.
 
-Hint Resolve fclosed_felift : term_db.
-Hint Resolve fclosed_fesubs : term_db.
+Hint Resolve closed_felift : term_db.
+Hint Resolve closed_fesubs : term_db.
 
 
 (** Proofs *)
@@ -113,26 +113,25 @@ Proof. now apply rnprove_mutrect; intros; try (econstructor; eassumption). Qed.
 (** * Normalization *)
 
 (** apply [r] on normal form *)
-Theorem rnpesubs r (Hc : fclosed r) {l A} :
+Theorem rnpesubs r (Hc : rclosed r) {l A} :
    (nprove l A -> nprove (map (esubs r) l) A⟦r⟧)
  * (rprove l A -> rprove (map (esubs r) l) A⟦r⟧).
 Proof.
 revert l A.
-enough ((forall l A, nprove l A -> forall r, fclosed r -> nprove (map (esubs r) l) A⟦r⟧)
-      * (forall l A, rprove l A -> forall r, fclosed r -> rprove (map (esubs r) l) A⟦r⟧))
+enough ((forall l A, nprove l A -> forall r, rclosed r -> nprove (map (esubs r) l) A⟦r⟧)
+      * (forall l A, rprove l A -> forall r, rclosed r -> rprove (map (esubs r) l) A⟦r⟧))
   as He by (split; intros; apply He; assumption).
 clear r Hc; apply rnprove_mutrect; intros; (try simpl in X);
   (try assert (IH1 := X r H)); (try assert (IH2 := X0 r H));
   (try (econstructor; (eassumption + intuition); fail)).
-- rewrite map_app; apply nax.
-- rcauto; rnow apply nfrle.
+- rewrite map_app. apply nax.
+- rcauto. rnow apply nfrle.
 - specialize X with (↑r0).
-  revert X; rcauto.
-  rewrite map_map, <- (map_ext _ _ (felift_esubs (evar 0) _)), <- map_map in X; intuition.
+  revert X. rcauto.
+  rewrite map_map, (map_ext _ _ (felift_esubs (evar 0) _)), <- map_map in X. intuition.
 Qed.
 
-Lemma rpsubsz {l A x u} : closed u ->
-  rprove l⇈ A↑[evar 0//x] -> rprove l (subs x u A).
+Lemma rpsubsz {l A x u} : closed u -> rprove l⇈ A↑[evar 0//x] -> rprove l (subs x u A).
 Proof.
 intros Hc pi.
 apply (rnpesubs (u⇓)) in pi; [ | intuition ].
