nj1_frl_ar.v
@@ -18,7 +18,7 @@ Arguments tvar {_} {_} {_} {T} _.
 
 Notation term := (@term vatom tatom tarity nat).
 Notation closed t := (tvars t = nil).
-Notation fclosed r := (forall n, closed (r n)).
+Notation rclosed r := (forall n, closed (r n)).
 Notation "↑ r" := (felift (evar 0) r) (at level 25, format "↑ r").
 Notation "v ⇓" := (fesubs v) (at level 18, format "v ⇓").
 Notation "A ⟦ r ⟧" := (esubs r A) (at level 8, left associativity, format "A ⟦ r ⟧").
@@ -34,14 +34,14 @@ Notation formula := (@formula vatom tatom tarity fatom farity Nocon Nocon Icon F
 
 Hint Rewrite (@fsize_esubs vatom tatom tarity fatom farity Nocon Nocon Icon FQcon) : term_db.
 Hint Rewrite (@fsize_subs vatom tatom tarity fatom farity Nocon Nocon Icon FQcon nat) : term_db.
-Hint Rewrite (@tvars_tesubs_fclosed vatom tatom tarity) using intuition; fail : term_db.
+Hint Rewrite (@tvars_tesubs_closed vatom tatom tarity) using intuition; fail : term_db.
 Hint Rewrite (@subs_esubs vatom tatom tarity fatom farity Nocon Nocon Icon FQcon nat)
                          using intuition; fail : term_db.
-Hint Rewrite <- (@felift_esubs vatom tatom tarity fatom farity Nocon Nocon Icon FQcon) : term_db.
+Hint Rewrite (@felift_esubs vatom tatom tarity fatom farity Nocon Nocon Icon FQcon) : term_db.
 Hint Rewrite (@esubs_fup vatom tatom tarity fatom farity Nocon Nocon Icon FQcon) : term_db.
 
-Hint Resolve fclosed_felift : term_db.
-Hint Resolve fclosed_fesubs : term_db.
+Hint Resolve closed_felift : term_db.
+Hint Resolve closed_fesubs : term_db.
 
 
 (** Proofs *)
@@ -114,13 +114,13 @@ Proof. now apply rnprove_mutrect; intros; try (econstructor; eassumption). Qed.
 (** * Normalization *)
 
 (** apply [r] on normal form *)
-Theorem rnpesubs r (Hc : fclosed r) {l A} :
+Theorem rnpesubs r (Hc : rclosed r) {l A} :
    (nprove l A -> nprove (map (esubs r) l) A⟦r⟧)
  * (rprove l A -> rprove (map (esubs r) l) A⟦r⟧).
 Proof.
 revert l A.
-enough ((forall l A, nprove l A -> forall r, fclosed r -> nprove (map (esubs r) l) A⟦r⟧)
-      * (forall l A, rprove l A -> forall r, fclosed r -> rprove (map (esubs r) l) A⟦r⟧))
+enough ((forall l A, nprove l A -> forall r, rclosed r -> nprove (map (esubs r) l) A⟦r⟧)
+      * (forall l A, rprove l A -> forall r, rclosed r -> rprove (map (esubs r) l) A⟦r⟧))
   as He by (split; intros; apply He; assumption).
 clear r Hc; apply rnprove_mutrect; intros; (try simpl in X);
   (try assert (IH1 := X r H)); (try assert (IH2 := X0 r H));
@@ -129,7 +129,7 @@ clear r Hc; apply rnprove_mutrect; intros; (try simpl in X);
 - rcauto; rnow apply nfrle.
 - specialize X with (↑r0).
   revert X; rcauto.
-  rewrite map_map, <- (map_ext _ _ (felift_esubs (evar 0) _)), <- map_map in X; intuition.
+  rewrite map_map, (map_ext _ _ (felift_esubs (evar 0) _)), <- map_map in X. intuition.
 Qed.
 
 Lemma rpsubsz {l A x u} : closed u ->
@@ -148,8 +148,7 @@ Proof.
 apply rnprove_mutrect; intros; subst;
   try (econstructor; rewrite_all map_app; rewrite ? app_comm_cons; intuition; fail).
 destruct (dichot_elt_app_inf _ _ _ _ _ H) as [ [? [? ?]] | [? [? ?]] ]; subst;
-  rewrite ? (app_assoc _ _ (A::_)), <- ? (app_assoc _ (A::_)), <- ? app_comm_cons;
-  intuition.
+  rewrite ? (app_assoc _ _ (A::_)), <- ? (app_assoc _ (A::_)), <- ? app_comm_cons; intuition.
 Qed.
 
 Lemma substitution : forall l A B, rprove l A -> rprove (A :: l) B -> rprove l B.
@@ -266,8 +265,8 @@ replace (fconstr (k:=0) (tconstr (tconstr (evar 0) (tfun nat f)) (tfun nat f)) (
    with (subs x (tconstr (evar 0) (tfun nat f))
         (fconstr (tconstr (tvar _ x) (tfun nat f)) (frel nat P : formula 1)))
   by rcauto.
-apply nfrle; auto.
-rewrite <- (app_nil_l (_ :: _)) ; apply nax.
+apply nfrle; [ reflexivity | ].
+rewrite <- (app_nil_l (_ :: _)). apply nax.
 Qed.
 
 End Examples.
